theories/ScopedProgramming/cterm.v
@@ -33,6 +33,12 @@ Obligation 1.
   simpl. auto.
 Defined.
 
+Program Definition cLambda :forall {n:nat}, aname -> cterm n -> cterm (S n) -> cterm n :=
+  fun n na t1 t2 => existc (tLambda na (proj1_sig t1) (proj1_sig t2)).
+Next Obligation.
+  destruct t1, t2. auto.
+Qed.
+
 Program Fixpoint cApp {n:nat} (x:cterm n) (yl:list (cterm n)) {struct yl}:
   cterm n :=
     match yl with
@@ -42,4 +48,66 @@ Program Fixpoint cApp {n:nat} (x:cterm n) (yl:list (cterm n)) {struct yl}:
   .
 Next Obligation. destruct x. auto. Qed.
 Next Obligation. destruct x, y. auto. Qed.
+
+
+(********************************************)
+(*not really used term*)
+
+Program Definition cVar {n:nat} ident : cterm n := existc (tVar ident).
+
+Program Definition cEvar {n:nat} (m:nat) (yl:list (cterm n)) : cterm n :=
+  existc (tEvar m (map (fun t => proj1_sig t) yl)).
+Next Obligation.
+  eapply forallb_Forall.
+  apply Forall_forall.
+  intro. intro.
+  induction yl.
+  - auto.
+  - simpl in H. destruct H.
+    + destruct a. simpl in H. rewrite <- H. auto.
+    + auto.
+Qed.
+
+Program Definition cSort {n:nat} sort : cterm n := existc (tSort sort).
+
+Program Definition cCast {n:nat} (c:cterm n) (ck:cast_kind) (t:cterm n) : cterm n :=
+  existc (tCast (proj1_sig c) ck (proj1_sig t)).
+Next Obligation.
+  destruct c, t. auto.
+Qed.
+
+Program Definition cLetIn {n:nat} na (b:cterm n) (t0:cterm n) (b':cterm (S n)) : cterm n :=
+  existc (tLetIn na (proj1_sig b) (proj1_sig t0) (proj1_sig b')).
+Next Obligation. destruct b, t0, b'. auto. Qed.
+
+Program Definition cConst {n:nat} kn instance : cterm n := existc (tConst kn instance).
+
+Program Definition cInd {n:nat} inductive instance : cterm n := existc (tInd inductive instance).
+
+Program Definition cConstruct {n:nat} inductive m instance : cterm n := existc (tConstruct inductive m instance).
+
+(* Program Definition cCase {n:nat} (ci:case_info) (p: c brs *)
+
+Program Definition cProj {n} projection (t:cterm n) : cterm n := existc (tProj projection (proj1_sig t)).
+Next Obligation. destruct t. auto. Qed.
+
+(* Program Definition cFix {n} *)
+
+(* Program Definition cCoFix {n}  *)
+
+Program Definition cInt {n} i : cterm n := existc (tInt i).
+
+Program Definition cFloat {n} f : cterm n := existc (tFloat f).
+
+Program Definition cArray {n:nat} level (arr:list (cterm n)) (def:cterm n) (ty:cterm n) : cterm n :=
+  existc (tArray level (map (fun t => proj1_sig t) arr) (proj1_sig def) (proj1_sig ty) ).
+Next Obligation.
+  destruct def, ty.
+  simpl.
+  assert (forallb (closedn n) (map (fun t : {t : term | closedn n t} => proj1_sig t) arr)).
+  - apply forallb_Forall. apply Forall_forall.
+    intros. induction arr.
+    + auto. + destruct H. ++ destruct a. simpl in H. rewrite <- H. auto. ++ auto.
+  - auto.
+Qed.
 
